examples/bytestring/prims_verif.v
@@ -61,11 +61,36 @@ The command has indeed failed with message:
 Tactic failure: Your Gprog contains no funspec with the name
 _get_Coq_Strings_String_string_tag (level 98).
 *)
- Admitted.
+   admit.
+ - change (Tpointer _ _) with int_or_ptr_type.
+   forward.
+   change (Tpointer _ _) with int_or_ptr_type.
+   forward.
+   forward.
+   deadvars!.
+   eapply semax_seq'.
+  +
+   eapply semax_Delta_subsumption with GC_SAVE1_tycontext.
+   apply prove_tycontext_sub; try reflexivity; repeat split; auto.
+   apply (@semax_cssub filteredCompSpecs).
+   apply prove_cssub; repeat split; auto; try reflexivity.
+   match goal with |- context [full_gc _ _ _ _ ?ti _ _] =>
+    match goal with |- context [temp ?tix ti] =>
+      change tix with specs_general._tinfo
+    end end.
 
-(* REMAINDER OF THIS FILE DUPLICATED FROM examples/uint63nat/prims_verif.v *)
-
-#[export] Instance CCE: change_composite_env env_graph_gc.CompSpecs CompSpecs.
-make_cs_preserve env_graph_gc.CompSpecs CompSpecs.
-Defined.
-
+  match goal with |- semax _ (PROPx ?P (LOCALx ?Q (SEPx ?R))) _ (normal_ret_assert ?Post) =>
+  let Q1 := get_rep_temps _tinfo Q in
+  let Q2 := get_nonrep_temps _tinfo Q in
+  let R1 := get_gc_mpreds R in
+  let R2 := get_nongc_mpreds R in
+(* apply_semax_GC_SAVE1. *)
+ eapply (semax_frame_PQR'' Q1 Q2 R1 R2); 
+  [solve [auto 50 with closed] 
+  | solve [go_lowerx; autorewrite with norm; cancel]
+  | apply perhaps_gc_1_live_root_aux
+  | (*eapply semax_GC_SAVE1; eauto*) ]
+ end.
+(* PROBLEM: GC_SAVE1 has a constant n, but here we have a variable _nalloc. *)
+ 
+Abort.
